$$
\begin{align}
{\psi}_1 &=1 - \left(\frac{x'_{E}}{L_{E}}\right)\\
{\psi}_2 &= 1 - 3\left(\frac{x'_E}{L_E}\right)^2 + 2\left(\frac{x'_E}{L_E}\right)^3\\
{\psi}_3 &= L_{E} \left[\left(\frac{x'_{E}}{L_{E}}\right) - 2\left(\frac{ x'_{E}}{L_{E}}\right)^{2} + \left(\frac{x'_{E}}{L_{E}}\right)^{3}\right]\\
{\psi}_4 &=\frac{x'_{E}}{L_{E}}\\
{\psi}_5 &=3 {\left(\frac{ x'_{E}}{L_{E}}\right)}^{2} -2 \left( \frac{ x'_{E}}{L_{E}}\right)^{3}\\
{\psi}_6 &=L_{E} \left[- \left(\frac{x'_{E}}{L_{E}}\right)^{2} + \left(\frac{x'_{E}}{L_{E}}\right)^{3}\right]
\end{align}
$$

